\documentclass[hidelinks,12pt]{article}
\usepackage[a4paper,width=150mm,top=25mm,bottom=25mm]{geometry}
\usepackage[utf8]{inputenc}
\usepackage{graphicx}
\usepackage{amsmath}
\usepackage{amssymb}
\usepackage{apacite}
\usepackage{natbib}
\usepackage{hyperref}
\usepackage{float}
\usepackage{ragged2e}
\usepackage[font={footnotesize,bf}]{caption}
\usepackage[nottoc,numbib]{tocbibind}
\usepackage{multirow}

\linespread{1.5}

\begin{document}

\begin{titlepage}
    \begin{center}
        \vspace*{1cm}
        
        
        % \vfill
        
        \large
        \textbf{Big Data Asset Pricing \\ Exercise 1: Beta-Dollar Neutral Portfolio Construction}
            
        
        \normalsize
        Seyyed Morteza Aghajanzadeh \\
        Department of Finance \\
        Stockholm School of Economics
        
        \vfill
        \normalsize
        \justifying
        \noindent
        \textbf{Statement:} I certify with my signature that I have solved the exercise according to the Code of Professional Conduct and Ethics. 
        For example, I have not plagiarized others, but, instead, solved the exercise myself (possibly with allowed collaboration with other students), and I have referenced my sources appropriately.

        \vfill
        
        \vspace{0.8cm}
            
        
        \vspace{0.8cm}
        \normalsize
        \centering
        2024-01
            
    \end{center}
\end{titlepage}
\section{}
The optimization problem is as follows:
\begin{equation*}
    \begin{aligned}
        & \underset{x }{\min}
        & & (x-y)^{'} (x-y) \\
        & s.t. 
        & & x^{'} \overrightarrow{1} = 0  \\
        & & & x^{'} \beta = 0
    \end{aligned}
\end{equation*}
where $x$ is the vector of weights of the portfolio, $y$ is the vector of weights of the benchmark. This problem would modify the benchmark portfolio in a way that the new portfolio is dollar and beta neutral.  The first constraint is the dollar neutrality constraint and the second constraint is the beta neutrality constraint.

\section{}
\begin{equation*}
    \begin{aligned}
        & \underset{x }{\min}
        & & (x-y)^{'} (x-y) \\
        & s.t. 
        & & x^{'} B = 0 
    \end{aligned}
\end{equation*}
\begin{equation*}
    \begin{aligned}
    &\Rightarrow \mathcal{L} = x^{'} x - x^{'} y - y^{'} x + y^{'} y +  x^{'} B \lambda^{'}\\
    F.O.C& \Rightarrow 2x - y - y - B \lambda^{'} = 0 \Rightarrow x = y + \frac{1}{2} B \lambda^{'} 
\end{aligned}
\end{equation*}
Now we can plug the solution for $x$ in the constraint and solve for $\lambda$:
\begin{equation*}
    \begin{aligned}
        & x^{'} B = 0 \\
        & \Rightarrow (y + \frac{1}{2} B \lambda^{'})^{'} B = 0 \\
        & \Rightarrow y^{'} B + \frac{1}{2} \lambda B^{'} B = 0 \\
        & \Rightarrow \lambda = -2 y^{'} B (B^{'} B)^{-1} \\
        & \Rightarrow x = y - B (B B^{'})^{-1} B^{'} y
    \end{aligned}
\end{equation*}




\end{document}